Construct the natural numbers inside VBG set theory.

examples/set-theory/vbg/vbgsetScript.sml
@@ -1,9 +1,12 @@
 open HolKernel boolLib bossLib Parse
+open lcsymtacs
+open boolSimps
 
 val _ = new_theory "vbgset"
 
 (* hide constants from the existing (typed) set theory *)
-val _ = app (ignore o hide) ["UNION", "IN", "SUBSET", "EMPTY", "INSERT"]
+val _ = app (ignore o hide) ["UNION", "IN", "SUBSET", "EMPTY", "INSERT",
+                             "CROSS", "INTER", "BIGINTER", "BIGUNION"]
 
 (* create a new type (of VBG classes) *)
 val _ = new_type("vbgc", 0)
@@ -145,7 +148,7 @@ val PCLASS_SINGC_EMPTY = store_thm(
 val SET_IN_SINGC = store_thm(
   "SET_IN_SINGC",
   ``SET a ⇒ (x ∈ SINGC a ⇔ (x = a))``,
-  SRW_TAC [boolSimps.CONJ_ss][SINGC_def, SPEC0]);
+  SRW_TAC [CONJ_ss][SINGC_def, SPEC0]);
 
 val SINGC_11 = store_thm(
   "SINGC_11",
@@ -172,7 +175,7 @@ val PCLASS_PAIRC_EMPTY = store_thm(
 val SET_IN_PAIRC = store_thm(
   "SET_IN_PAIRC",
   ``SET a ∧ SET b ⇒ (∀x. x ∈ PAIRC a b ⇔ (x = a) ∨ (x = b))``,
-  SRW_TAC [boolSimps.CONJ_ss, boolSimps.DNF_ss][PAIRC_def, SPEC0]);
+  SRW_TAC [CONJ_ss, DNF_ss][PAIRC_def, SPEC0]);
 
 val UNORDERED_PAIRS = new_axiom(
   "UNORDERED_PAIRS",
@@ -222,14 +225,19 @@ val UNIONS = new_axiom(
 
 val UNION_SET_CLOSED = store_thm(
   "UNION_SET_CLOSED",
-  ``SET A ∧ SET B ⇒ SET (A ∪ B)``,
-  STRIP_TAC THEN
-  `SET (PAIRC A B)` by METIS_TAC [PAIRC_SET_CLOSED] THEN
-  POP_ASSUM (STRIP_ASSUME_TAC o MATCH_MP UNIONS) THEN
-  POP_ASSUM MP_TAC THEN
-  ASM_SIMP_TAC (srw_ss() ++ boolSimps.DNF_ss)[SET_IN_PAIRC] THEN
-  STRIP_TAC THEN MATCH_MP_TAC SUBSETS_ARE_SETS THEN Q.EXISTS_TAC `w` THEN
-  SRW_TAC [][SUBSET_def] THEN SRW_TAC [][]);
+  ``SET (A ∪ B) ⇔ SET A ∧ SET B``,
+  Tactical.REVERSE EQ_TAC >| [
+    STRIP_TAC THEN
+    `SET (PAIRC A B)` by METIS_TAC [PAIRC_SET_CLOSED] THEN
+    POP_ASSUM (STRIP_ASSUME_TAC o MATCH_MP UNIONS) THEN
+    POP_ASSUM MP_TAC THEN
+    ASM_SIMP_TAC (srw_ss() ++ DNF_ss)[SET_IN_PAIRC] THEN
+    STRIP_TAC THEN MATCH_MP_TAC SUBSETS_ARE_SETS THEN Q.EXISTS_TAC `w` THEN
+    SRW_TAC [][SUBSET_def] THEN SRW_TAC [][],
+    strip_tac >> conj_tac >> match_mp_tac SUBSETS_ARE_SETS >>
+    qexists_tac `A ∪ B` >> srw_tac [][SUBSET_def]
+  ]);
+val _ = export_rewrites ["UNION_SET_CLOSED"]
 
 val BIGUNION_SET_CLOSED = store_thm(
   "BIGUNION_SET_CLOSED",
@@ -237,6 +245,26 @@ val BIGUNION_SET_CLOSED = store_thm(
   STRIP_TAC THEN IMP_RES_TAC UNIONS THEN MATCH_MP_TAC SUBSETS_ARE_SETS THEN
   Q.EXISTS_TAC `w` THEN ASM_SIMP_TAC (srw_ss()) [SUBSET_def] THEN
   METIS_TAC []);
+
+(* intersections *)
+val INTER_def = Define`
+  s1 INTER s2 = SPEC0 (λe. e ∈ s1 ∧ e ∈ s2)
+`;
+
+val IN_INTER = store_thm(
+  "IN_INTER",
+  ``e ∈ s1 ∩ s2 ⇔ SET e ∧ e ∈ s1 ∧ e ∈ s2``,
+  rw [INTER_def, SPEC0]);
+val _ = export_rewrites ["IN_INTER"]
+
+val INTER_SET_CLOSED = store_thm(
+  "INTER_SET_CLOSED",
+  ``(SET s1 ⇒ SET (s1 ∩ s2)) ∧ (SET s2 ⇒ SET (s1 ∩ s2))``,
+  rpt strip_tac >> match_mp_tac SUBSETS_ARE_SETS >| [
+    qexists_tac `s1`,
+    qexists_tac `s2`
+  ] >> rw[SUBSET_def]);
+val _ = export_rewrites ["INTER_SET_CLOSED"]
 
 val INSERT_def = Define`x INSERT y = SINGC x ∪ y`
 
@@ -250,11 +278,7 @@ val _ = export_rewrites ["IN_INSERT"]
 val SET_INSERT = store_thm(
   "SET_INSERT",
   ``SET (x INSERT b) = SET b``,
-  SRW_TAC [][INSERT_def] THEN
-  Cases_on `SET b` THEN1 SRW_TAC [][UNION_SET_CLOSED] THEN
-  SRW_TAC [][] THEN
-  Q_TAC SUFF_TAC `b ⊆ SINGC x ∪ b` THEN1 METIS_TAC [SUBSETS_ARE_SETS] THEN
-  SRW_TAC [][SUBSET_def]);
+  SRW_TAC [][INSERT_def])
 val _ = export_rewrites ["SET_INSERT"]
 
 val INSERT_IDEM = store_thm(
@@ -292,18 +316,18 @@ val BIGUNION_SING = store_thm(
 val BIGUNION_UNION = store_thm(
   "BIGUNION_UNION",
   ``SET a ∧ SET b ⇒ (BIGUNION {a;b} = a ∪ b)``,
-  SRW_TAC [boolSimps.DNF_ss][Once EXTENSION]);
+  SRW_TAC [DNF_ss][Once EXTENSION]);
 
 val POW_EMPTY = store_thm(
   "POW_EMPTY",
   ``POW {} = {{}}``,
-  SRW_TAC [][Once EXTENSION] THEN SRW_TAC [boolSimps.CONJ_ss][]);
+  SRW_TAC [][Once EXTENSION] THEN SRW_TAC [CONJ_ss][]);
 
 val POW_SING = store_thm(
   "POW_SING",
   ``SET a ⇒ (POW {a} = {{}; {a}})``,
   SRW_TAC [][Once EXTENSION] THEN
-  ASM_SIMP_TAC (srw_ss() ++ boolSimps.CONJ_ss ++ boolSimps.DNF_ss) [] THEN
+  ASM_SIMP_TAC (srw_ss() ++ CONJ_ss ++ DNF_ss) [] THEN
   METIS_TAC []);
 
 (* "primitive ordered pair" *)
@@ -351,17 +375,17 @@ val OPAIR_def = Define`
 val SET_OPAIR = store_thm(
   "SET_OPAIR",
   ``SET a ∧ SET b ⇒ SET (OPAIR a b)``,
-  SRW_TAC [][OPAIR_def] THEN MATCH_MP_TAC UNION_SET_CLOSED THEN CONJ_TAC THENL[
+  SRW_TAC [][OPAIR_def] THENL[
     SRW_TAC [][POPAIR_def] THEN MATCH_MP_TAC SUBSETS_ARE_SETS THEN
-    SRW_TAC [boolSimps.DNF_ss][SUBSET_def, SPEC0] THEN
+    SRW_TAC [DNF_ss][SUBSET_def, SPEC0] THEN
     Q.EXISTS_TAC `POW (POW (a ∪ {{}}))` THEN
-    SRW_TAC [][POW_SET_CLOSED, UNION_SET_CLOSED] THEN
-    ASM_SIMP_TAC (srw_ss() ++ boolSimps.DNF_ss) [SUBSET_def],
+    SRW_TAC [][POW_SET_CLOSED] THEN
+    ASM_SIMP_TAC (srw_ss() ++ DNF_ss) [SUBSET_def],
     SRW_TAC [][POPAIR_def] THEN MATCH_MP_TAC SUBSETS_ARE_SETS THEN
-    SRW_TAC [boolSimps.DNF_ss][SUBSET_def, SPEC0] THEN
+    SRW_TAC [DNF_ss][SUBSET_def, SPEC0] THEN
     Q.EXISTS_TAC `POW (POW (b ∪ {{{}}}))` THEN
-    SRW_TAC [][POW_SET_CLOSED, UNION_SET_CLOSED] THEN
-    ASM_SIMP_TAC (srw_ss() ++ boolSimps.DNF_ss) [SUBSET_def]
+    SRW_TAC [][POW_SET_CLOSED] THEN
+    ASM_SIMP_TAC (srw_ss() ++ DNF_ss) [SUBSET_def]
   ]);
 
 val ZERO_NEQ_ONE = store_thm(
@@ -423,6 +447,187 @@ val _ = add_rule { fixity = Closefix,
                    pp_elements = [TOK "〈", TM, HardSpace 1,
                                   TOK "·", BreakSpace(1,2),
                                   TM, TOK "〉"]}
+
+val CROSS_def = Define`
+  s1 CROSS s2 = SPEC0 (λx. ∃a b. a ∈ s1 ∧ b ∈ s2 ∧ (x = 〈a · b〉))
+`;
+
+val FunSpace_def = Define`
+  FunSpace A B = SPEC0 (λf. f ⊆ A × B ∧ ∀a. a ∈ A ⇒ ∃!b. 〈a · b〉 ∈ f)
+`
+
+val id_def = Define`
+  id A = SPEC0 (λx. ∃a. a ∈ A ∧ (x = 〈a·a〉))
+`;
+
+(*
+val apply_def = new_specification("apply_def",
+  ["apply"],
+  CONV_RULE SKOLEM_CONV
+            (prove(``∀f x A B. f ∈ FunSpace A B ∧ x ∈ A ⇒
+                               ∃y. y ∈ B ∧ 〈x·y〉 ∈ f``,
+                   SRW_TAC [][FunSpace_def, SPEC0, CROSS_def] THEN
+                   RES_TAC THEN
+                   FULL_SIMP_TAC (srw_ss()) [EXISTS_UNIQUE_THM] THEN
+                   Q.EXISTS_TAC `b` THEN SRW_TAC [][] THEN
+                   FULL_SIMP_TAC (srw_ss()) [SUBSET_def, SPEC0] THEN
+                   RES_TAC THEN FULL_SIMP_TAC (srw_ss()) [OPAIR_11])
+*)
+
+val vSUC_def = Define`vSUC x = x ∪ {x}`
+
+val fromNat_def = Define`
+  (fromNat 0 = {}) ∧
+  (fromNat (SUC n) = vSUC (fromNat n))
+`;
+val _ = add_numeral_form(#"v", SOME "fromNat")
+
+val inductive_def = Define`
+  inductive A ⇔ SET A ∧ {} ∈ A ∧ ∀x. x ∈ A ⇒ vSUC x ∈ A
+`;
+
+val Inductives_def = Define`
+  Inductives = SPEC0 (λA. {} ∈ A ∧ ∀x. x ∈ A ⇒ vSUC x ∈ A)
+`;
+
+val inductive_Inductives = store_thm(
+  "inductive_Inductives",
+  ``inductive A ⇔ A ∈ Inductives``,
+  srw_tac [][inductive_def, Inductives_def, SPEC0]);
+
+val Nats_def = Define`
+  Nats = SPEC0 (λn. ∀s. inductive s ⇒ n ∈ s)
+`;
+
+val EMPTY_IN_Nats = store_thm(
+  "EMPTY_IN_Nats",
+  ``{} ∈ Nats``,
+  rw [Nats_def, SPEC0, inductive_def]);
+
+val vSUC_IN_Nats = store_thm(
+  "vSUC_IN_Nats",
+  ``n ∈ Nats ⇒ vSUC n ∈ Nats``,
+  rw [Nats_def, SPEC0, inductive_def, vSUC_def]);
+
+val SET_fromNat = store_thm(
+  "SET_fromNat",
+  ``SET (fromNat n)``,
+  Induct_on `n` >> srw_tac [][fromNat_def, vSUC_def]);
+val _ = export_rewrites ["SET_fromNat"]
+
+val fromNat_in_Nats = store_thm(
+  "fromNat_in_Nats",
+  ``∀n. fromNat n ∈ Nats``,
+  Induct THEN SRW_TAC [][fromNat_def] THENL [
+    SRW_TAC [][Nats_def, SPEC0] THEN
+    fs [inductive_def],
+    fs [Nats_def, SPEC0, vSUC_def] >>
+    fs [inductive_def, vSUC_def]
+  ]);
+
+val NOT_IN_0 = store_thm(
+  "NOT_IN_0",
+  ``x ∉ 0``,
+  SRW_TAC [][fromNat_def]);
+val _ = export_rewrites ["NOT_IN_0"]
+
+val vSUC_NOT_0 = store_thm(
+  "vSUC_not_0",
+  ``vSUC n ≠ 0``,
+  SRW_TAC [][vSUC_def, EXTENSION] THEN
+  Cases_on `n = 0` THEN SRW_TAC [][] THENL [
+    Q.EXISTS_TAC `0` THEN SRW_TAC [][],
+    METIS_TAC [fromNat_def, EMPTY_UNIQUE]
+  ]);
+
+val Nats_SET = store_thm(
+  "Nats_SET",
+  ``SET Nats``,
+  match_mp_tac SUBSETS_ARE_SETS >>
+  strip_assume_tac INFINITY >>
+  qexists_tac `w` >> simp [SUBSET_def] >>
+  qx_gen_tac `n` >> rw [Nats_def, SPEC0] >>
+  first_assum match_mp_tac >> simp [inductive_def] >> conj_tac
+    >- metis_tac [EMPTY_UNIQUE] >>
+  qx_gen_tac `e` >> strip_tac >>
+  `∃y. y ∈ w ∧ ∀u. u ∈ y ⇔ u ∈ e ∨ (u = e)` by metis_tac[] >>
+  qsuff_tac `vSUC e = y` >- rw[] >>
+  rw [vSUC_def, Once EXTENSION] >> metis_tac [SET_def]);
+
+val Nats_inductive = store_thm(
+  "Nats_inductive",
+  ``Nats ∈ Inductives``,
+  rw [SPEC0, SUBSET_def, Inductives_def, Nats_SET, EMPTY_IN_Nats,
+      vSUC_IN_Nats]);
+
+val Nats_least_inductive = store_thm(
+  "Nats_least_inductive",
+  ``P ∈ Inductives ⇒ Nats ⊆ P``,
+  rw[Inductives_def, SPEC0, SUBSET_def] >>
+  fs [Nats_def, SPEC0, inductive_def])
+
+val Nats_SETs = prove(``n ∈ Nats ⇒ SET n``, metis_tac [SET_def])
+val _ = augment_srw_ss [rewrites [Nats_SETs]]
+(*
+Higher order logic wins here: can capture all possible predicates.
+Can simplify to membership of a set S by making the predicate P be just that.
+ ⊢ ∀P. P {} ∧ (∀x. P x ∧ x ∈ Nats ⇒ P (vSUC x)) ⇒ ∀u. u ∈ Nats ⇒ P u
+*)
+val nat_induction = save_thm(
+  "nat_induction",
+  Nats_least_inductive
+      |> SIMP_RULE(srw_ss())[SUBSET_def,Inductives_def,SPEC0]
+      |> Q.GEN `P`
+      |> Q.SPEC `SPEC0 P ∩ Nats`
+      |> SIMP_RULE (srw_ss() ++ CONJ_ss)
+                   [Nats_SET, EMPTY_IN_Nats, vSUC_IN_Nats, SPEC0]
+      |> Q.GEN `P`);
+
+val transitive_def = Define`
+  transitive X ⇔ ∀x. x ∈ X ⇒ x ⊆ X
+`;
+
+val transitive_ALT = store_thm(
+  "transitive_ALT",
+  ``transitive X ⇔ ∀x y. x ∈ y ∧ y ∈ X ⇒ x ∈ X``,
+  rw [transitive_def] >> metis_tac [SUBSET_def]);
+
+val Nats_transitive = store_thm(
+  "Nats_transitive",
+  ``∀n. n ∈ Nats ⇒ transitive n``,
+  ho_match_mp_tac nat_induction >> conj_tac >> rw[transitive_def] >>
+  fs [vSUC_def, SUBSET_def] >> metis_tac []);
+
+val Nats_not_selfmembers = store_thm(
+  "Nats_not_selfmembers",
+  ``∀n. n ∈ Nats ⇒ n ∉ n``,
+  ho_match_mp_tac nat_induction >> rw[vSUC_def] >| [
+    strip_tac >> `n ∈ n ∪ {n}` by rw[] >>
+    metis_tac [Nats_transitive, transitive_ALT],
+    rw[Once EXTENSION] >> metis_tac []
+  ]);
+
+val pre_IN_vSUC = store_thm(
+  "pre_IN_vSUC",
+  ``SET n ⇒ n ∈ vSUC n``,
+  rw[vSUC_def]);
+
+val SET_vSUC = store_thm(
+  "SET_vSUC",
+  ``SET (vSUC n) = SET n``,
+  rw[vSUC_def, EQ_IMP_THM]);
+val _ = export_rewrites ["SET_vSUC"]
+
+val vSUC_11 = store_thm(
+  "vSUC_11",
+  ``∀n m. n ∈ Nats ∧ m ∈ Nats ⇒ ((vSUC n = vSUC m) ⇔ (n = m))``,
+  rw[EQ_IMP_THM] >>
+  `n ∈ vSUC m` by metis_tac [pre_IN_vSUC, SET_vSUC, Nats_SETs] >>
+  pop_assum mp_tac >> rw[vSUC_def] >>
+  `m ∈ vSUC n` by metis_tac [pre_IN_vSUC, SET_vSUC, Nats_SETs] >>
+  fs[vSUC_def] >>
+  metis_tac [transitive_ALT, Nats_transitive, Nats_not_selfmembers]);
+
 
 (*
 val FORMATION = new_axiom(
